---
abbrlink: a14030c
categories: Math example
tags: Math Example

---
### $1^\infty型结论运用$

$eg 1.\lim\limits_{n\to \infty}\frac{n^{n+1}}{(n+1)^n}\sin \frac{1}{n} 
\newline 思路：转变成 \lim(1+\alpha(x))^{\beta(x)}的形式,且满足\lim\alpha(x)=0,\lim\beta(x)=\infty .\newline所以上述可以写为 \newline  \qquad \lim\limits_{n\to \infty} n \cdot (\frac{n}{n+1})^n \cdot \sin\frac{1}{n} 
\newline \because \lim\limits_{n\to \infty}(\frac{n}{n+1})^n=\lim\limits_{n\to \infty}(1+(-\frac{1}{n+1}))^n\xRightarrow{use \ conclusion}\lim\limits_{n\to \infty}-\frac{1}{n+1}\cdot n=-1 \newline
\therefore \lim\limits_{n\to \infty}(\frac{n}{n+1})^n=e^{-1} 
\newline and \ \lim\limits_{x\to \infty}n\cdot\sin\frac{1}{n}=\lim\limits_{x\to 0}\frac{\sin n}{n}=1 
\newline  \therefore\lim\limits_{n\to \infty}\frac{n^{n+1}}{(n+1)^n}\sin \frac{1}{n} =e^{-1}$

<br>

$eg 2.\lim\limits_{x\to 0^{+}}(\cos\sqrt{x})^{\frac{\pi}{x}}
\newline =\lim\limits_{x\to 0^+}((\cos\sqrt x -1)+1)^\frac{\pi}{x} \mskip{3em}\text{accoring to above method}
\newline \lim\alpha(x)\beta(x) = \lim\limits_{x\to 0^+}(\cos\sqrt x-1)\cdot \frac{\pi}{x}=-\frac{\pi}{2} \mskip{2em} \text{Taylor expansion or Replacement}
\newline \therefore \lim\limits_{x\to 0^+}(\cos\sqrt{x})^{\frac{\pi}{x}}=e^{-\frac{\pi}{2}}$
 
 $eg3.\lim\limits_{x\to \infty} (\frac{\sqrt[n]a+\sqrt[n]{b}+\sqrt[n]{c}}{3})^n \qquad  \ a,b,c>0
 \newline=\lim\limits_{x\to \infty}(\frac{\sqrt[n]{a}+\sqrt[n]{b}+\sqrt[n]{c}}{3}-1+1)^n
 \newline \therefore \lim\limits_{x\to \infty} (\frac{\sqrt[n]{a}+\sqrt[n]{b}+\sqrt[n]{c}}{3}-1)\cdot n
 \newline=\lim\limits_{x\to 0}\frac{1}{3}(\frac{a^n-1}{n}+\frac{b^n-1}{n}+\frac{c^n-1}{n})\newline=\frac{\ln a+\ln b +\ln c}{3}=\frac{1}{3}\ln abc$
 $\therefore\lim\limits_{x\to \infty}(\frac{\sqrt[n]a+\sqrt[n]{b}+\sqrt[n]{c}}{3})^n=e^{\frac{1}{3}\ln abc}=\sqrt[3]{abc}$
   
 $eg4.\lim\limits_{x\to \frac{\pi}{4}}(\tan x)^{\frac{1}{\cos x -\sin x}}
 \newline=\lim\limits_{x\to \frac{\pi}{4}}(\tan x -1 +1)^{\frac{1}{\cos x -sin x}}\newline
 \therefore \lim\limits_{x\to \frac{\pi}{4}}(\tan x-1)\cdot \frac{1}{\cos x- \sin x}=\lim\limits_{x\to \frac{\pi}{4}}(\tan x-1)\frac{1}{\cos x(1-tanx)}=\lim\limits_{x\to \frac{\pi}{4}}-\frac{1}{cosx}=-\sqrt2
 \newline\therefore\lim\limits_{x\to \frac{\pi}{4}}(tanx)^\frac{1}{cosx -sinx}=e^{-\sqrt2}$

$eg5.$

-------
### Equivalent substitution

$eg6. \lim\limits_{x\to \infty}(\frac{x^2}{(x-a)(x+b)})^x
\newline =\lim\limits_{x\to \infty}(\frac{x}{x-a}\cdot \frac{x}{x+b})^x=\lim\limits_{x\to \infty}(\frac{x}{x-a})^x\cdot (\frac{x}{x+b})^x
\newline=\lim\limits_{x\to \infty}(1-\frac{a}{x})^{-x}\cdot (1+\frac{b}{x})^{-x}  \qquad \text{twice conclusion}
\newline = \lim\limits_{x\to \infty}e^{a}\cdot e^{-b}=e^{a-b}$

$eg7. \lim\limits_{x\to 0}\frac{\sqrt{1+f(x)\sin 2x}-1}{e^{3x}-1}=2,\quad so \ \lim\limits_{x\to 0}f(x)=?
\newline  \because e^{3x}-1\backsim 3x,\ (1+x)^{\alpha}-1\backsim \alpha x  \qquad\text{if x-> 0} \newline \textcolor{red}{tips:\ x \ could\ be\ a \ func,\ like \ f(x),but \ precondition:  \lim\limits_{x\to 0} f(x)=0}
\newline \therefore \sqrt{1+f(x)sin2x}-1\backsim \frac{1}{2}f(x)sin2x\backsim \frac{1}{2}f(x)2x
\newline so \lim\limits_{x\to 0}\frac{\sqrt{1+f(x)\sin 2x}-1}{e^{3x}-1}=\lim\limits_{x\to 0}\frac{\frac{1}{2}f(x)2x}{3x}=\lim\limits_{x\to 0}\frac{f(x)x}{3x}=\lim\limits_{x\to0}\frac{f(x)}{3}=2
\newline \qquad \therefore \lim\limits_{x\to 0}f(x)=6$

$eg8. \lim\limits_{x\to 0}\frac{\ln(\cos x)}{x^2} \newline
=\lim\limits_{x\to 0}\frac{\ln ([cosx-1]+1)}{x^2}=\lim\limits_{x\to 0}\frac{cosx-1}{x^2}=\lim\limits_{x\to 0}\frac{-\frac{1}{2}x^2}{x^2}=-\frac{1}{2} \qquad Replacement  :\ ln(f(x)+1)\backsim f(x) \qquad  if \  \lim\limits_{x\to 0}f(x)=0$

$eg9. \lim\limits_{x\to 0}\frac{e-e^{cosx}}{\sqrt[3]{1+x^2}-1}\newline
=\lim\limits_{x\to 0}\frac{e(1-e^{cosx-1})}{\frac{1}{3}x^2}=e\cdot\lim\limits_{x\to 0}\frac{1-e^{-\frac{1}{2}x^2}}{\frac{1}{3}x^2}=e\cdot \lim\limits_{x\to 0}\frac{\frac{1}{2}x^2}{\frac{1}{3}x^2}=\frac{3e}{2}\newline \because ({1+x^2})^{\frac{1}{3}}-1\backsim \frac{1}{3}x^2,\ e^x-1\backsim x,\ cosx-1\backsim \frac{1}{2}x^2$

$eg10. \lim\limits_{x\to 0}\frac{1}{x^3}[(\frac{2+cosx}{3})^x-1]
\newline=\lim\limits_{x\to 0}\frac{1}{x^3}[xln(\frac{2+cosx}{3})] =\lim\limits_{x\to 0}\frac{ln([\frac{(2+cosx)}{3}-1]+1)}{x^2}=\lim\limits_{x\to 0}\frac{cosx-1}{3}\cdot\frac{1}{x^2}=-\frac{1}{6}
\newline \because \alpha ^x-1\backsim xlna,\ cosx-1\backsim -\frac{1}{2}x^2 ,\ ln(x+1)\backsim x$

$eg11. \lim\limits_{x\to 0}\frac{arcsinx-sinx}{arctanx-tanx}\newline=\lim\limits_{x\to 0}\frac{[arcsinx-x]-[sinx-x]}{[arctanx-x]-[tanx-x]}$

$eg12. \lim\limits_{x\to 0}\frac{(1-cosx)[x-ln(1+tanx)]}{\sin^{4}x} \newline
=\lim\limits_{x\to 0}\frac{\frac{1}{2}x^2[x-tanx]}{x^{4}}=\frac{\frac{1}{2}[x-tanx]}{x^2}$

$eg13. \lim\limits_{x\to 0}[\frac{1}{x}-(\frac{1}{x}-a)e^x]=1 ,\qquad a=?
\newline\lim\limits_{x\to 0}[\frac{1-e^x}{x}+ae^x]=\lim\limits_{x\to 0}-1+a=1
\newline \qquad \therefore a=2$

$eg14. \lim\limits_{x\to +\infty}[(ax+b)e^{\frac{1}{x}}-x]=2, \qquad a,b=?
\newline =\lim\limits_{x\to 0}[(\frac{a}{x}+b)e^x-\frac{1}{x}]=\lim\limits_{x\to 0}[\frac{ae^x-1}{x}]+\lim\limits_{x\to 0}be^x=1+b=2
\newline \therefore a=b=1 \mskip{3em}\textcolor{blue}{\newline According \ to\ basic\ four\ algorithm\ rule,\newline if\   \ \lim f(x)g(x)=a  \ \&\&\exist \  \lim f(x),there \ must \ be \ \exist \ \lim g(x)  }$

$eg15.\lim\limits_{x\to -\infty}\frac{\sqrt{4x^2+x-1}+x+1}{\sqrt{x^2+sinx}}
\newline=\lim\limits_{x\to -\infty}\frac{-x\cdot(\sqrt{4+\frac{1}{x}-\frac{1}{x^2}}-1-\frac{1}{x})}{-x\cdot\sqrt{1+\frac{sinx}{x^2}}}=
\lim\limits_{x\to -\infty}\frac{2-1-0}{1}=1
\newline \textcolor{orange}{the\ key\ point\ is\ eliminating\ the\ infty\  factor\ }$

-----
### Law of Robida
$eg16:\lim\limits_{x\to 1}(1-x^2)\tan \frac{\pi}{2}x \qquad type:0\cdot\infty
\newline= \lim\limits_{x\to 1}(x+1)(x-1)\cdot\frac{sin\frac{\pi}{2}x}{cos\frac{\pi}{2}x} \qquad \because \lim\limits_{x\to 1}(x+1)=2,\lim\limits_{x\to 1}sin(\frac{\pi}{2}x)=1.
\newline  =\lim\limits_{x\to 1}\frac{x-1}{cos\frac{\pi}{2}x}=\lim\limits_{x\to 1}\frac{1}{-\frac{\pi}{2}\cdot sin\frac{\pi}{2}x}=-\frac{2}{\pi}$

$eg17. \lim\limits_{x\to 1}\frac{ln(cosx-1)}{1-sin\frac{\pi}{2}x} \qquad type:\frac{0}{0}
\newline=\lim\limits_{x\to 1}\frac{-\tan (x-1)}{-\frac{\pi}{2}cos\frac{\pi}{2}x}=\lim\limits_{x\to 1}\frac{-(x-1)}{-\frac{\pi}{2}cos\frac{\pi}{2}x} \qquad if \ x-1\to  0, \ have\ tan(x-1)\backsim x-1 
\newline =-\frac{2}{\pi}\lim\limits_{x\to 1}\frac{1}{\frac{\pi}{2}\cdot sin\frac{\pi}{2}x}=-\frac{4}{\pi^{2}}$

$eg18.\lim\limits_{x\to +\infty}(x+\sqrt{1+x^2})^\frac{1}{x}\qquad tpye:\infty ^0
\newline =\lim\limits_{x\to +\infty}e^{\frac{1}{x}ln(x+\sqrt{1+x^2})}=\lim\limits_{x\to +\infty}e^{\frac{\infty}{\infty}}=\lim\limits_{x\to +\infty}e^{\frac{1}{\sqrt{1+x^2}}}=e^0=1$

### Taylor Expansion

$eg19. \lim\limits_{x\to 0}\frac{\cos x-e^{-\frac{x^2}{2}}}{x^4}
\newline \because \lim\limits_{x\to 0}\cos x=1-\frac{1}{2}x^2+\frac{1}{24}x^4+o(x^4), \quad \lim\limits_{x\to 0}e^x=1+x+\frac{1}{2}x^2+\frac{1}{6}x^3+\frac{1}{24}x^4+o(x^4)
\newline \therefore \lim\limits_{x\to 0}\frac{\cos x-e^{-\frac{x^2}{2}}}{x^4}=-\frac{1}{12}$

$eg20. \lim\limits_{x\to 0}\frac{\ln (1+x)-(ax+bx^2)}{x^2}=2 \qquad a,b=?
\newline \because \lim\limits_{x\to 0}\ln (1+x)=0+x+-\frac{1}{2}x^2+o(x^2)
\newline \therefore a=1, b=-\frac{5}{2}$

$eg21. \lim\limits_{x\to 0}\frac{\sin 6x+xf(x)}{x^3}=0  \qquad \lim\limits_{x\to 0}\frac{6+f(x)}{x^2}=?
\newline \because \lim\limits_{x\to 0}\sin x=x-\frac{1}{6}x^3+o(x^3)
\newline \therefore\lim\limits_{x\to 0}\frac{\sin 6x+xf(x)}{x^3}=\lim\limits_{x\to 0}\frac{x(6+f(x))-36x^3}{x^3}=0 \Rightarrow  \lim\limits_{x\to 0} \frac{6+f(x)}{x^2}-36=0
\newline \therefore \lim\limits_{x\to 0}\frac{6+f(x)}{x^2}=36$


$eg22. x\to 9,\alpha(x)=kx^2,\beta(x)=\sqrt{1+x\arcsin x}-\sqrt{\cos x} \ are\  equivalent\ ,k=?
\newline \textcolor{red}{way \ one: Rationalisation}
\newline \quad \lim\limits_{x\to 0}\frac{\sqrt{1+x\arcsin x}-\sqrt{\cos x}}{kx^2} \qquad type:\frac{0}{0}
\newline= \lim\limits_{x\to 0}\frac{1+x\arcsin x -cosx}{kx^2[\sqrt{1+x\arcsin x}+\sqrt{\cos x} ]}
\newline=\frac{1}{2}  \lim\limits_{x\to 0}\frac{1+x\arcsin x -cosx}{kx^2} = \frac{1}{2}\frac{x^2+\frac{1}{2}x^2}{kx^2}=\frac{3}{4k}=1
\newline \therefore k=\frac{4}{3}
\newline \textcolor{red}{way \ two :\ Lagrange's\ mean\ value\ theorem}
\newline \quad\lim\limits_{x\to 0}\frac{\sqrt{1+x\arcsin x}-\sqrt{\cos x}}{kx^2} \qquad f(x)=\sqrt{x}
\newline =\lim\limits_{x\to 0}\frac{\frac{1}{2\xi}[1+arcsin x-cos x]}{kx^2}=1 \rightarrow k=\frac{4}{3}
\newline\textcolor{red}{way \ three :\ Equivalent \ Replacement}
\newline \quad\lim\limits_{x\to 0}\frac{\sqrt{1+x\arcsin x}-\sqrt{\cos x}}{kx^2} \qquad 
\newline   =\lim\limits_{x\to 0}\frac{[\sqrt{1+x\arcsin x}-1]-[\sqrt{\cos x-1+1}-1]}{kx^2}=\lim\limits_{x\to 0}\frac{\frac{1}{2}[x\arcsin x-(cosx-1)]}{kx^2}=1
\newline \therefore k=\frac{4}{3}
$

